Weidenbach_Book/IsaSAT/IsaSAT_Setup1_LLVM.thy
@@ -4,55 +4,242 @@ theory IsaSAT_Setup1_LLVM
 begin
 
 
-(*TODO proper setup to test if the conflict is none*)
-sepref_def get_conflict_wl_is_None_fast_code
-  is \<open>RETURN o get_conflict_wl_is_None_heur\<close>
-  :: \<open>isasat_bounded_assn\<^sup>k \<rightarrow>\<^sub>a bool1_assn\<close>
-  unfolding get_conflict_wl_is_None_heur_alt_def isasat_bounded_assn_def length_ll_def[symmetric]
-    conflict_option_rel_assn_def
-  supply [[goals_limit=1]]
+context
+  fixes C :: \<open>64 word\<close> and C' :: nat
+begin
+
+definition not_deleted_code where
+  \<open>not_deleted_code xi = do\<^sub>M {
+  x \<leftarrow> arena_status_impl xi C;
+  status_neq_impl x 3
+  }\<close>
+
+
+context
+  assumes [sepref_import_param]: \<open>(C, C') \<in> snat_rel' TYPE(64)\<close>
+  notes [[sepref_register_adhoc C']]
+begin
+
+sepref_register arena_status DELETED
+qualified sepref_definition not_deleted_code_tmp
+  is \<open>(\<lambda>N. do {status \<leftarrow> RETURN (arena_status N C'); RETURN (status \<noteq> DELETED)})\<close>
+  :: \<open>[\<lambda>N. arena_is_valid_clause_vdom N C']\<^sub>a arena_fast_assn\<^sup>k \<rightarrow> bool1_assn\<close>
   by sepref
 
+lemmas not_deleted_code_refine =
+  not_deleted_code_tmp.refine[unfolded not_deleted_code_tmp_def
+    not_deleted_code_def[symmetric]]
+end
+end
 
-sepref_def isa_count_decided_st_fast_code
-  is \<open>RETURN o isa_count_decided_st\<close>
-  :: \<open>isasat_bounded_assn\<^sup>k \<rightarrow>\<^sub>a uint32_nat_assn\<close>
-  supply [[goals_limit=2]]
-  unfolding isa_count_decided_st_def isasat_bounded_assn_def
+lemma clause_not_marked_to_delete_heur_alt_def:
+  \<open>RETURN oo clause_not_marked_to_delete_heur = (\<lambda> S C'. read_arena_wl_heur (\<lambda>N. do {status \<leftarrow> RETURN (arena_status N C'); RETURN (status \<noteq> DELETED)}) S)\<close>
+  by (auto intro!: ext simp: clause_not_marked_to_delete_heur_def read_arena_wl_heur_def
+    split: isasat_int.splits)
+
+definition clause_not_marked_to_delete_heur_code :: \<open>twl_st_wll_trail_fast2 \<Rightarrow> _ \<Rightarrow> _\<close> where
+  \<open>clause_not_marked_to_delete_heur_code S C' = read_arena_wl_heur_code (not_deleted_code C') S\<close>
+
+global_interpretation arena_is_valid: read_arena_param_adder where
+  R = \<open>snat_rel' TYPE(64)\<close> and
+  f = \<open>\<lambda>C N. (not_deleted_code C) N\<close> and
+  f' = \<open>(\<lambda>C' N. do {status \<leftarrow> RETURN (arena_status N C'); RETURN (status \<noteq> DELETED)})\<close> and
+  x_assn = bool1_assn and
+  P = \<open>(\<lambda>C S. arena_is_valid_clause_vdom S C)\<close>
+  rewrites \<open>(\<lambda>S C'. read_arena_wl_heur (\<lambda>N. do {status \<leftarrow> RETURN (arena_status N C'); RETURN (status \<noteq> DELETED)}) S) = RETURN oo clause_not_marked_to_delete_heur\<close> and
+  \<open>(\<lambda>S C'. read_arena_wl_heur_code (not_deleted_code C') S) = clause_not_marked_to_delete_heur_code\<close>
+  apply unfold_locales
+  apply (rule not_deleted_code_refine; assumption)
+  unfolding clause_not_marked_to_delete_heur_alt_def clause_not_marked_to_delete_heur_code_def
+  by (solves \<open>rule refl\<close>)+
+
+sepref_register clause_not_marked_to_delete_heur
+lemmas [sepref_fr_rules] = arena_is_valid.refine
+lemmas [llvm_code] = clause_not_marked_to_delete_heur_code_def[unfolded read_arena_wl_heur_code_def not_deleted_code_def]
+
+definition conflict_is_None  :: \<open>conflict_option_rel \<Rightarrow> bool nres\<close> where
+  \<open>conflict_is_None =(\<lambda>N. do {let (b, _) = N;  RETURN b})\<close>
+definition \<open>conflict_is_None_code :: option_lookup_clause_assn \<Rightarrow> 1 word llM \<equiv>
+\<lambda>(a, _). do\<^sub>M {
+  return\<^sub>M (a)
+  }\<close>
+lemma conflict_is_None_code_refine[sepref_fr_rules] :
+  \<open>(conflict_is_None_code, conflict_is_None) \<in> conflict_option_rel_assn\<^sup>k \<rightarrow>\<^sub>a bool1_assn\<close>
+  unfolding conflict_is_None_code_def conflict_is_None_def Let_def conflict_option_rel_assn_def
+  apply sepref_to_hoare
+  apply vcg
+  done
+
+lemma get_conflict_wl_is_None_heur_alt_def: \<open>read_conflict_wl_heur conflict_is_None = RETURN \<circ> get_conflict_wl_is_None_heur\<close>
+  by (auto simp: read_conflict_wl_heur_def get_conflict_wl_is_None_heur_def conflict_is_None_def
+    intro!: ext split: isasat_int.splits)
+
+definition get_conflict_wl_is_None_heur2 where
+  \<open>get_conflict_wl_is_None_heur2 = RETURN o get_conflict_wl_is_None_heur\<close>
+
+
+definition get_conflict_wl_is_None_fast_code :: \<open>twl_st_wll_trail_fast2 \<Rightarrow> _\<close> where
+  \<open>get_conflict_wl_is_None_fast_code = read_conflict_wl_heur_code conflict_is_None_code\<close>
+
+global_interpretation conflict_is_None: read_conflict_param_adder0 where
+  f = \<open>conflict_is_None_code\<close> and
+  f' = \<open>conflict_is_None\<close> and
+  x_assn = bool1_assn and
+  P = \<open>(\<lambda>S. True)\<close>
+  rewrites \<open>(\<lambda>S. read_conflict_wl_heur (conflict_is_None) S) = get_conflict_wl_is_None_heur2\<close> and
+  \<open>(\<lambda>S. read_conflict_wl_heur_code (conflict_is_None_code) S) = get_conflict_wl_is_None_fast_code\<close>
+  apply unfold_locales
+  apply (rule conflict_is_None_code_refine; assumption)
+  unfolding get_conflict_wl_is_None_heur2_def get_conflict_wl_is_None_fast_code_def
+  by (solves \<open>rule get_conflict_wl_is_None_heur_alt_def refl\<close>)+
+thm inline_return_node_case
+
+lemmas [sepref_fr_rules] = conflict_is_None.refine[unfolded get_conflict_wl_is_None_heur2_def]
+lemmas [llvm_code] = conflict_is_None_code_def
+lemmas [unfolded inline_direct_return_node_case, llvm_code] =
+  get_conflict_wl_is_None_fast_code_def[unfolded read_conflict_wl_heur_code_def]
+
+llvm_deps get_conflict_wl_is_None_fast_code
+export_llvm get_conflict_wl_is_None_fast_code
+
+
+lemma count_decided_st_heur_alt_def:
+  \<open>RETURN o count_decided_st_heur = read_trail_wl_heur (RETURN \<circ> count_decided_pol)\<close>
+  by (auto intro!: ext simp: count_decided_st_heur_def count_decided_pol_def
+    read_trail_wl_heur_def split: isasat_int.splits)
+
+definition count_decided_st_heur_impl where
+  \<open>count_decided_st_heur_impl = read_trail_wl_heur_code count_decided_pol_impl\<close>
+
+sepref_register extract_trail_wl_heur count_decided_pol update_trail_wl_heur count_decided_st_heur
+
+lemma lambda_comp_true: \<open>(\<lambda>S. True) \<circ> f = (\<lambda>_. True)\<close> \<open>uncurry (\<lambda>a b. True) = (\<lambda>_. True)\<close>
+  by auto
+
+lemmas [llvm_code] =
+  read_trail_wl_heur_code_def
+
+definition isa_count_decided_st_fast_code :: \<open>twl_st_wll_trail_fast2 \<Rightarrow> _\<close> where
+  \<open>isa_count_decided_st_fast_code = read_trail_wl_heur_code count_decided_pol_impl\<close>
+
+lemmas [sepref_fr_rules] =
+  read_trail_wl_heur_code_refine[OF count_decided_pol_impl.refine, unfolded count_decided_st_heur_alt_def[symmetric]
+  lambda_comp_true isa_count_decided_st_fast_code_def[symmetric]]
+
+
+global_interpretation count_decided: read_trail_param_adder0 where
+  f = \<open>count_decided_pol_impl\<close> and
+  f' = \<open>RETURN o count_decided_pol\<close> and
+  x_assn = uint32_nat_assn and
+  P = \<open>(\<lambda>S. True)\<close>
+  rewrites \<open>read_trail_wl_heur (RETURN o count_decided_pol) = RETURN o isa_count_decided_st\<close> and
+  \<open>read_trail_wl_heur_code count_decided_pol_impl = isa_count_decided_st_fast_code\<close>
+  apply unfold_locales
+  apply (rule count_decided_pol_impl.refine)
+  subgoal
+    by (auto simp: read_trail_wl_heur_def isa_count_decided_st_def intro!: ext
+      split: isasat_int.splits)
+  subgoal
+    by (auto simp: isa_count_decided_st_fast_code_def)
+  done
+
+lemmas [sepref_fr_rules] = count_decided.refine[unfolded lambda_comp_true]
+lemmas [unfolded inline_direct_return_node_case, llvm_code] =
+  isa_count_decided_st_fast_code_def[unfolded read_trail_wl_heur_code_def]
+
+definition polarity_st_heur_pol_fast ::  \<open>twl_st_wll_trail_fast2 \<Rightarrow> _\<close>  where
+  \<open>polarity_st_heur_pol_fast = (\<lambda>S C. read_trail_wl_heur_code (\<lambda>L. polarity_pol_fast L C) S)\<close>
+
+global_interpretation mop_count_decided: read_trail_param_adder where
+  f = \<open>\<lambda>S L. polarity_pol_fast L S\<close> and
+  f' = \<open>\<lambda>S L. mop_polarity_pol L S\<close> and
+  x_assn = tri_bool_assn and
+  P = \<open>\<lambda>S _. True\<close> and
+  R = \<open>unat_lit_rel\<close>
+  rewrites \<open>(\<lambda>S C. read_trail_wl_heur_code (\<lambda>L. polarity_pol_fast L C) S) = polarity_st_heur_pol_fast\<close> and
+  \<open>(\<lambda>S C'. read_trail_wl_heur (\<lambda>L. mop_polarity_pol L C') S) = mop_polarity_st_heur\<close>
+  apply unfold_locales
+  apply (rule remove_pure_parameter2[where f = polarity_pol_fast and f' = mop_polarity_pol])
+  apply (subst lambda_comp_true)
+  apply (rule polarity_pol_fast.refine)
+  apply assumption
+  subgoal
+    by (auto simp: polarity_st_heur_pol_fast_def)
+  subgoal
+    by (auto simp: mop_polarity_st_heur_def read_trail_wl_heur_def
+      split: isasat_int.splits intro!: ext)
+  done
+
+lemmas [sepref_fr_rules] = mop_count_decided.refine[unfolded lambda_comp_true]
+lemmas [unfolded inline_direct_return_node_case, llvm_code] =
+  polarity_st_heur_pol_fast_def[unfolded read_trail_wl_heur_code_def]
+
+definition arena_lit2 where \<open>arena_lit2 N i j = arena_lit N (i+j)\<close>
+
+sepref_def arena_lit2_impl
+  is \<open>uncurry2 (RETURN ooo arena_lit2)\<close>
+    :: \<open>[uncurry2 (\<lambda>N i j. arena_lit_pre N (i+j) \<and> length N \<le> sint64_max)]\<^sub>a arena_fast_assn\<^sup>k *\<^sub>a sint64_nat_assn\<^sup>k *\<^sub>a sint64_nat_assn\<^sup>k \<rightarrow> unat_lit_assn\<close>
+  supply [dest] = arena_lit_implI
+  unfolding arena_lit_def arena_lit2_def
   by sepref
 
-sepref_def polarity_st_heur_pol_fast
-  is \<open>uncurry (mop_polarity_st_heur)\<close>
-  :: \<open>isasat_bounded_assn\<^sup>k *\<^sub>a unat_lit_assn\<^sup>k \<rightarrow>\<^sub>a tri_bool_assn\<close>
-  unfolding mop_polarity_st_heur_alt_def isasat_bounded_assn_def polarity_st_pre_def
-    mop_polarity_st_heur_alt_def
-  supply [[goals_limit = 1]]
-  by sepref
+lemma arena_lit2_impl_arena_lit:
+  assumes \<open>(C, C') \<in> snat_rel\<close> and
+    \<open>(D, D') \<in> snat_rel\<close>
+  shows \<open>(\<lambda>S. arena_lit2_impl S C D, \<lambda>S. RETURN (arena_lit S (C' + D')))
+    \<in> [\<lambda>S. arena_lit_pre S (C' + D') \<and> length S \<le> sint64_max]\<^sub>a (al_assn arena_el_impl_assn)\<^sup>k \<rightarrow> unat_lit_assn\<close>
+proof -
+  have arena_lit2: \<open>RETURN ooo arena_lit2 = (\<lambda>S C' D'. RETURN (arena_lit2 S C' D'))\<close> for f
+    by (auto intro!: ext)
+  show ?thesis
+  apply (rule remove_pure_parameter2_twoargs[where R = \<open>snat_rel' TYPE(64)\<close> and f = \<open>\<lambda>a C D. arena_lit2_impl a C D\<close> and f' =
+     \<open>\<lambda>S C' D'. RETURN (arena_lit S (C' + D'))\<close>, OF _ assms])
+  unfolding arena_lit2_def[symmetric] arena_lit2[symmetric]
+  by (rule arena_lit2_impl.refine)
+qed
+
+lemma access_lit_in_clauses_heur_alt_def:
+  \<open>RETURN ooo access_lit_in_clauses_heur = (\<lambda>N C' D. read_arena_wl_heur (\<lambda>N. RETURN (arena_lit N (C' + D))) N)\<close>
+  by (auto intro!: ext simp: read_arena_wl_heur_def access_lit_in_clauses_heur_def split: isasat_int.splits)
+
+lemma access_lit_in_clauses_heur_pre:
+  \<open>uncurry2
+   (\<lambda>S C D.
+    arena_lit_pre (get_clauses_wl_heur S) (C + D) \<and>
+    length (get_clauses_wl_heur S) \<le> sint64_max) = uncurry2 (\<lambda>S i j. access_lit_in_clauses_heur_pre ((S, i), j) \<and>
+           length (get_clauses_wl_heur S) \<le> sint64_max)\<close>
+  by (auto simp: access_lit_in_clauses_heur_pre_def)
+
+definition access_lit_in_clauses_heur_fast_code :: \<open>twl_st_wll_trail_fast2 \<Rightarrow> _ \<Rightarrow> _ \<Rightarrow> _\<close> where
+  \<open>access_lit_in_clauses_heur_fast_code = (\<lambda>N C D. read_arena_wl_heur_code (\<lambda>N. arena_lit2_impl N C D) N)\<close>
+
+global_interpretation access_arena: read_arena_param_adder2_twoargs' where
+  R = \<open>(snat_rel' TYPE(64))\<close> and
+  R' = \<open>snat_rel' TYPE(64)\<close> and
+  f' = \<open>\<lambda>N i j. RETURN (arena_lit N (i+j))\<close> and
+  f = \<open>arena_lit2_impl\<close> and
+  x_assn = unat_lit_assn and
+  P = \<open>(\<lambda>i j S. arena_lit_pre (S) (i+j) \<and> length S \<le> sint64_max)\<close>
+  rewrites
+     \<open>(\<lambda>N C' D. read_arena_wl_heur (\<lambda>N. RETURN (arena_lit N (C' + D))) N) = RETURN ooo access_lit_in_clauses_heur\<close> and
+    \<open>(\<lambda>N C D. read_arena_wl_heur_code (\<lambda>N. arena_lit2_impl N C D) N) = access_lit_in_clauses_heur_fast_code\<close> and
+  \<open>uncurry2 (\<lambda>S C D. arena_lit_pre (get_clauses_wl_heur S) (C + D) \<and> length (get_clauses_wl_heur S) \<le> sint64_max) =
+    uncurry2 (\<lambda>S i j. access_lit_in_clauses_heur_pre ((S, i), j) \<and> length (get_clauses_wl_heur S) \<le> sint64_max)\<close>
+  apply unfold_locales
+  apply (rule arena_lit2_impl_arena_lit; assumption)
+  apply (subst access_lit_in_clauses_heur_alt_def; rule refl)
+  apply (subst access_lit_in_clauses_heur_fast_code_def; rule refl)
+  apply (rule access_lit_in_clauses_heur_pre)
+  done
+
+lemmas [sepref_fr_rules] = access_arena.refine
+
+lemmas [unfolded inline_direct_return_node_case, llvm_code] =
+  access_lit_in_clauses_heur_fast_code_def[unfolded read_arena_wl_heur_code_def]
 
 
-subsection \<open>More theorems\<close>
 
-sepref_def count_decided_st_heur_pol_fast
-  is \<open>RETURN o count_decided_st_heur\<close>
-  :: \<open>isasat_bounded_assn\<^sup>k \<rightarrow>\<^sub>a uint32_nat_assn\<close>
-  unfolding isasat_bounded_assn_def count_decided_st_heur_alt_def fold_tuple_optimizations
-  supply [[goals_limit = 1]]
-  by sepref
-
-setup \<open>map_theory_claset (fn ctxt => ctxt addSbefore ("split_all_tac", split_all_tac))\<close>
-sepref_def access_lit_in_clauses_heur_fast_code
-  is \<open>uncurry2 (RETURN ooo access_lit_in_clauses_heur)\<close>
-  :: \<open>[\<lambda>((S, i), j). access_lit_in_clauses_heur_pre ((S, i), j) \<and>
-           length (get_clauses_wl_heur S) \<le> sint64_max]\<^sub>a
-      isasat_bounded_assn\<^sup>k *\<^sub>a sint64_nat_assn\<^sup>k  *\<^sub>a sint64_nat_assn\<^sup>k \<rightarrow> unat_lit_assn\<close>
-  supply [[goals_limit=1]] arena_lit_pre_le[dest]
-  unfolding isasat_bounded_assn_def access_lit_in_clauses_heur_alt_def
-    access_lit_in_clauses_heur_pre_def
-  unfolding fold_tuple_optimizations
-  by sepref
-
-setup \<open>map_theory_claset (fn ctxt => ctxt delSWrapper ("split_all_tac"))\<close>
-
+sepref_register mop_arena_lit2 mop_arena_length mop_append_ll
 sepref_def rewatch_heur_vdom_fast_code
   is \<open>uncurry2 (rewatch_heur_vdom)\<close>
   :: \<open>[\<lambda>((vdom, arena), W). (\<forall>x \<in> set (get_tvdom_aivdom vdom). x \<le> sint64_max) \<and> length arena \<le> sint64_max \<and>
@@ -71,43 +258,116 @@ sepref_def rewatch_heur_vdom_fast_code
   apply (annot_snat_const \<open>TYPE(64)\<close>)
   by sepref
 
+lemma rewatch_heur_st_fast_alt_def:
+  \<open>rewatch_heur_st_fast = (\<lambda>S\<^sub>0. do {
+  let (N, S) = extract_arena_wl_heur S\<^sub>0;
+  let (W, S) = extract_watchlist_wl_heur S;
+  let (vdom, S) = extract_vdom_wl_heur S;
+  ASSERT(length (get_tvdom_aivdom vdom) \<le> length N);
+  ASSERT (vdom = get_aivdom S\<^sub>0);
+  ASSERT (N = get_clauses_wl_heur S\<^sub>0);
+  ASSERT (W = get_watched_wl_heur S\<^sub>0);
+  W \<leftarrow> rewatch_heur (get_tvdom_aivdom vdom) N W;
+  let S = update_arena_wl_heur N S;
+  let S = update_watchlist_wl_heur W S;
+  let S = update_vdom_wl_heur vdom S;
+  RETURN S
+  })\<close>
+  by (auto simp: rewatch_heur_st_fast_def rewatch_heur_st_def
+    extract_arena_wl_heur_def extract_watchlist_wl_heur_def extract_vdom_wl_heur_def
+    isasat_state_ops.remove_arena_wl_heur_def  isasat_state_ops.remove_watchlist_wl_heur_def  isasat_state_ops.remove_vdom_wl_heur_def
+    update_arena_wl_heur_def update_watchlist_wl_heur_def update_vdom_wl_heur_def
+    split: isasat_int.splits
+    intro!: ext)
+
+lemmas [sepref_fr_rules] =
+  remove_watchlist_wl_heur_code.refine
+  remove_vdom_wl_heur_code.refine
+  remove_arena_wl_heur_code.refine
 
 sepref_def rewatch_heur_st_fast_code
   is \<open>(rewatch_heur_st_fast)\<close>
   :: \<open>[rewatch_heur_st_fast_pre]\<^sub>a
        isasat_bounded_assn\<^sup>d \<rightarrow> isasat_bounded_assn\<close>
   supply [[goals_limit=1]]
-  unfolding rewatch_heur_st_def PR_CONST_def rewatch_heur_st_fast_pre_def
-    isasat_bounded_assn_def rewatch_heur_st_fast_def rewatch_heur_vdom_def[symmetric]
-  unfolding fold_tuple_optimizations
+  unfolding rewatch_heur_st_fast_alt_def rewatch_heur_st_def rewatch_heur_vdom_def[symmetric] rewatch_heur_st_fast_pre_def
   by sepref
 
+definition length_ivdom_fast_code :: \<open>twl_st_wll_trail_fast2 \<Rightarrow> _\<close> where
+  \<open>length_ivdom_fast_code = read_vdom_wl_heur_code length_ivdom_aivdom_impl\<close>
+global_interpretation length_ivdom_aivdom: read_vdom_param_adder0 where
+  f = \<open>length_ivdom_aivdom_impl\<close> and
+  f' = \<open>RETURN o length_ivdom_aivdom\<close> and
+  x_assn = sint64_nat_assn and
+  P = \<open>(\<lambda>S. True)\<close>
+  rewrites \<open>read_vdom_wl_heur (RETURN o length_ivdom_aivdom) = RETURN o length_ivdom\<close> and
+  \<open>read_vdom_wl_heur_code length_ivdom_aivdom_impl = length_ivdom_fast_code\<close>
+  apply unfold_locales
+  apply (rule vdom_ref)
+  subgoal
+    by (auto simp: read_vdom_wl_heur_def length_ivdom_aivdom_def length_ivdom_def intro!: ext
+      split: isasat_int.splits)
+  subgoal
+    by (auto simp: length_ivdom_fast_code_def)
+  done
+
+definition length_avdom_fast_code :: \<open>twl_st_wll_trail_fast2 \<Rightarrow> _\<close> where
+  \<open>length_avdom_fast_code = read_vdom_wl_heur_code length_avdom_aivdom_impl\<close>
+
+global_interpretation length_avdom_aivdom: read_vdom_param_adder0 where
+  f = \<open>length_avdom_aivdom_impl\<close> and
+  f' = \<open>RETURN o length_avdom_aivdom\<close> and
+  x_assn = sint64_nat_assn and
+  P = \<open>(\<lambda>S. True)\<close>
+  rewrites \<open>read_vdom_wl_heur (RETURN o length_avdom_aivdom) = RETURN o length_avdom\<close> and
+  \<open>read_vdom_wl_heur_code length_avdom_aivdom_impl = length_avdom_fast_code\<close>
+  apply unfold_locales
+  apply (rule vdom_ref)
+  subgoal
+    by (auto simp: read_vdom_wl_heur_def length_avdom_aivdom_def length_avdom_def intro!: ext
+      split: isasat_int.splits)
+  subgoal
+    by (auto simp: length_avdom_fast_code_def)
+  done
+
+
+definition length_tvdom_fast_code :: \<open>twl_st_wll_trail_fast2 \<Rightarrow> _\<close> where
+  \<open>length_tvdom_fast_code = read_vdom_wl_heur_code length_tvdom_aivdom_impl\<close>
+
+global_interpretation length_tvdom_aivdom: read_vdom_param_adder0 where
+  f = \<open>length_tvdom_aivdom_impl\<close> and
+  f' = \<open>RETURN o length_tvdom_aivdom\<close> and
+  x_assn = sint64_nat_assn and
+  P = \<open>(\<lambda>S. True)\<close>
+  rewrites \<open>read_vdom_wl_heur (RETURN o length_tvdom_aivdom) = RETURN o length_tvdom\<close> and
+  \<open>read_vdom_wl_heur_code length_tvdom_aivdom_impl = length_tvdom_fast_code\<close>
+  apply unfold_locales
+  apply (rule vdom_ref)
+  subgoal
+    by (auto simp: read_vdom_wl_heur_def length_tvdom_aivdom_def length_tvdom_def intro!: ext
+      split: isasat_int.splits)
+  subgoal
+    by (auto simp: length_tvdom_fast_code_def)
+  done
+
+
+lemmas [sepref_fr_rules] = length_ivdom_aivdom.refine[unfolded lambda_comp_true]
+  length_avdom_aivdom.refine[unfolded lambda_comp_true]
+  length_tvdom_aivdom.refine[unfolded lambda_comp_true]
+
+lemmas [unfolded inline_direct_return_node_case, llvm_code] =
+  length_ivdom_fast_code_def[unfolded read_vdom_wl_heur_code_def]
+  length_avdom_fast_code_def[unfolded read_vdom_wl_heur_code_def]
+  length_tvdom_fast_code_def[unfolded read_vdom_wl_heur_code_def]
 
 sepref_register length_avdom length_ivdom length_tvdom
 
-sepref_def length_avdom_fast_code
-  is \<open>RETURN o length_avdom\<close>
-  :: \<open>isasat_bounded_assn\<^sup>k \<rightarrow>\<^sub>a sint64_nat_assn\<close>
-  unfolding length_avdom_alt_def isasat_bounded_assn_def fold_tuple_optimizations
-    length_avdom_aivdom_def[symmetric]
-  supply [[goals_limit = 1]]
-  by sepref
+export_llvm polarity_st_heur_pol_fast isa_count_decided_st_fast_code get_conflict_wl_is_None_fast_code
+  clause_not_marked_to_delete_heur_code access_lit_in_clauses_heur_fast_code length_ivdom_fast_code
+  length_avdom_fast_code length_tvdom_fast_code
 
-sepref_def length_ivdom_fast_code
-  is \<open>RETURN o length_ivdom\<close>
-  :: \<open>isasat_bounded_assn\<^sup>k \<rightarrow>\<^sub>a sint64_nat_assn\<close>
-  unfolding length_ivdom_alt_def isasat_bounded_assn_def fold_tuple_optimizations
-    length_ivdom_aivdom_def[symmetric]
-  supply [[goals_limit = 1]]
-  by sepref
+subsection \<open>More theorems\<close>
 
-sepref_def length_tvdom_fast_code
-  is \<open>RETURN o length_tvdom\<close>
-  :: \<open>isasat_bounded_assn\<^sup>k \<rightarrow>\<^sub>a sint64_nat_assn\<close>
-  unfolding length_tvdom_alt_def isasat_bounded_assn_def fold_tuple_optimizations
-    length_tvdom_aivdom_def[symmetric]
-  supply [[goals_limit = 1]]
-  by sepref
  
 sepref_register get_the_propagation_reason_heur
 
